src/SlabsOverlay.fsti
@@ -1,0 +1,291 @@
+module SlabsOverlay
+
+open Utils2
+open Steel.Effect.Atomic
+open Steel.Effect
+open Steel.Reference
+module A = Steel.Array
+
+open Slabs
+
+module U64 = FStar.UInt64
+module U32 = FStar.UInt32
+module U8 = FStar.UInt8
+module SL = Selectors.LList
+
+module SM = Steel.Memory
+module G = FStar.Ghost
+
+val vrefinedep_hp
+  (v: vprop)
+  (p: ( (t_of v) -> Tot prop))
+  (f: ( t_of (vrefine v p) -> Tot vprop))
+  : Tot (SM.slprop u#1)
+
+[@__steel_reduce__]
+let vrefinedep_t
+  (v: vprop)
+  (p: ( (t_of v) -> Tot prop))
+  (f: ( t_of (vrefine v p) -> Tot vprop))
+  : Tot Type
+  =
+  dtuple2 (t_of (vrefine v p)) (fun x -> t_of (f x))
+
+val vrefinedep_sel
+  (v: vprop)
+  (p: ( (t_of v) -> Tot prop))
+  (f: ( (t_of (vrefine v p)) -> Tot vprop))
+  : Tot (selector (vrefinedep_t v p f) (vrefinedep_hp v p f))
+
+[@@__steel_reduce__]
+let vrefinedep'
+  (v: vprop)
+  (p: ( (t_of v) -> Tot prop))
+  (f: ( (t_of (vrefine v p)) -> Tot vprop))
+  : Tot vprop' = {
+  hp = vrefinedep_hp v p f;
+  t = vrefinedep_t v p f;
+  sel = vrefinedep_sel v p f;
+}
+[@@__steel_reduce__]
+let vrefinedep
+  (v: vprop)
+  (p: ( (t_of v) -> Tot prop))
+  (f: ( (t_of (vrefine v p)) -> Tot vprop))
+  = VUnit (vrefinedep' v p f)
+
+val elim_vrefinedep
+  (#opened:_)
+  (v: vprop)
+  (p: ( (t_of v) -> Tot prop))
+  (f: ( (t_of (vrefine v p)) -> Tot vprop))
+  : SteelGhost (G.erased (t_of (vrefine v p))) opened
+  (vrefinedep v p f)
+  (fun res -> v `star` f (G.reveal res))
+  (requires fun _ -> True)
+  (ensures fun h res h' ->
+    let (res : normal (t_of v){p res}) = res in
+    p res /\
+    G.reveal res == h' v /\
+    (let fs : x:t_of v{p x} = h' v in
+    let sn : t_of (f (G.reveal res)) = h' (f (G.reveal res)) in
+    let x2 = h (vrefinedep v p f) in
+    G.reveal res == fs /\
+    dfst x2 == fs /\
+    dsnd x2 == sn /\
+    True)
+  )
+
+val intro_vrefinedep
+  (#opened:_)
+  (v: vprop)
+  (p: ( (t_of v) -> Tot prop))
+  (f: ( (t_of (vrefine v p)) -> Tot vprop))
+  (f': vprop)
+  : SteelGhost unit opened
+  (v `star` f')
+  (fun _ -> vrefinedep v p f)
+  (requires fun h ->
+    p (h v) /\
+    f' == f (h v))
+  (ensures fun h _ h' ->
+    p (h v) /\
+    f' == f (h v) /\
+    (let x2 = h' (vrefinedep v p f) in
+    let sn : t_of f' = h f' in
+    dfst x2 == h v /\
+    dsnd x2 == sn)
+  )
+
+#push-options "--compat_pre_typed_indexed_effects"
+#push-options "--z3rlimit 20"
+let vrefinedep_idem
+  (#opened:_)
+  (v: vprop)
+  (p: ( (t_of v) -> Tot prop))
+  (f: ( (t_of (vrefine v p)) -> Tot vprop))
+  : SteelGhost unit opened
+  (vrefinedep v p f)
+  (fun _ -> vrefinedep v p f)
+  (requires fun _ -> True)
+  (ensures fun h _ h' ->
+    h (vrefinedep v p f)
+    ==
+    h' (vrefinedep v p f)
+  )
+  =
+  //let h0 = get () in
+  let x0 = gget (vrefinedep v p f) in
+  let x = elim_vrefinedep v p f in
+  intro_vrefinedep v p  f (f (G.reveal x));
+  //let h1 = get () in
+  let x1 = gget (vrefinedep v p f) in
+  assert (dfst x0 == dfst x1);
+  assert (dsnd x0 == dsnd x1);
+  //assert (x0 == x1);
+  ()
+#pop-options
+#pop-options
+
+open FStar.Mul
+
+// #push-options "--compat_pre_typed_indexed_effects --compat_pre_core 0"
+// val alloc_metadata2
+//   (size_class: sc)
+//   (slab_region: array U8.t{A.length slab_region = U32.v metadata_max * U32.v page_size})
+//   (md_bm_region: array U64.t{A.length md_bm_region = U32.v metadata_max * 4})
+//   (md_region: array (SL.cell blob){A.length md_region = U32.v metadata_max})
+//   (md_count: ref U32.t)
+//   : Steel (SL.t blob)
+//   //: Steel unit
+//   (
+//     vrefinedep
+//       (vptr md_count)
+//       //TODO: hideous coercion
+//       (fun x -> U32.v x < U32.v metadata_max == true)
+//       (fun v ->
+//         A.varray (A.split_r slab_region (u32_to_sz (U32.mul v page_size))) `star`
+//         A.varray (A.split_r md_bm_region (u32_to_sz (U32.mul v 4ul))) `star`
+//         A.varray (A.split_r md_region (u32_to_sz v)))
+//   )
+//   (fun r ->
+//     SL.llist (p_empty size_class) r `star`
+//     vrefinedep
+//       (vptr md_count)
+//       //TODO: hideous coercion
+//       (fun x -> U32.v x <= U32.v metadata_max == true)
+//       (fun v ->
+//         A.varray (A.split_r slab_region (u32_to_sz (U32.mul v page_size))) `star`
+//         A.varray (A.split_r md_bm_region (u32_to_sz (U32.mul v 4ul))) `star`
+//         A.varray (A.split_r md_region (u32_to_sz v)))
+//   )
+//   (requires fun h0 -> True)
+//   (ensures fun h0 r h1 -> True
+//     //TODO FIXME: fails with this postcondition
+//     // FStar.List.Tot.length (SL.v_llist (p_empty size_class) r h1) == 1
+// //    /\ sel md_count h1 = U32.add (sel md_count h0) 1ul
+//   )
+
+#push-options "--compat_pre_typed_indexed_effects --z3rlimit 100"
+let alloc_metadata2
+  (size_class: sc)
+  (slab_region: array U8.t{A.length slab_region = U32.v metadata_max * U32.v page_size})
+  (md_bm_region: array U64.t{A.length md_bm_region = U32.v metadata_max * 4})
+  (md_region: array (SL.cell blob){A.length md_region = U32.v metadata_max})
+  (md_count: ref U32.t)
+  : Steel (SL.t blob)
+  //: Steel unit
+  (
+    vrefinedep
+      (vptr md_count)
+      //TODO: hideous coercion
+      (fun x -> U32.v x < U32.v metadata_max == true)
+      (fun v ->
+        A.varray (A.split_r slab_region (u32_to_sz (U32.mul v page_size))) `star`
+        A.varray (A.split_r md_bm_region (u32_to_sz (U32.mul v 4ul))) `star`
+        A.varray (A.split_r md_region (u32_to_sz v)))
+  )
+  (fun r ->
+    SL.llist (p_empty size_class) r `star`
+    vrefinedep
+      (vptr md_count)
+      //TODO: hideous coercion
+      (fun x -> U32.v x <= U32.v metadata_max == true)
+      (fun v ->
+        A.varray (A.split_r slab_region (u32_to_sz (U32.mul v page_size))) `star`
+        A.varray (A.split_r md_bm_region (u32_to_sz (U32.mul v 4ul))) `star`
+        A.varray (A.split_r md_region (u32_to_sz v)))
+  )
+  (requires fun h0 -> True)
+  (ensures fun h0 r h1 -> True
+    //TODO FIXME: fails with this postcondition
+    //L.length (SL.v_llist (p_empty size_class) r h1) = 1
+    ///\ sel md_count h1 = U32.add (sel md_count h0) 1ul
+  )
+  =
+  let x
+    //: G.erased (x:U32.t{U32.v x < U32.v metadata_max == true})
+    = elim_vrefinedep
+    (vptr md_count)
+    (fun x -> U32.v x < U32.v metadata_max == true)
+    (fun v ->
+      A.varray (A.split_r slab_region (u32_to_sz (U32.mul v page_size))) `star`
+      A.varray (A.split_r md_bm_region (u32_to_sz (U32.mul v 4ul))) `star`
+      A.varray (A.split_r md_region (u32_to_sz v)))
+  in
+  let x'
+    : G.erased (x:U32.t{U32.v x < U32.v metadata_max})
+    = G.hide (G.reveal x <: x:U32.t{U32.v x < U32.v metadata_max}) in
+  //TODO: hideous coercion that leads to 2 change_slprop_rel
+  change_equal_slprop
+    (A.varray (A.split_r slab_region (u32_to_sz (U32.mul (G.reveal x) page_size))) `star`
+    A.varray (A.split_r md_bm_region (u32_to_sz (U32.mul (G.reveal x) 4ul))) `star`
+    A.varray (A.split_r md_region (u32_to_sz (G.reveal x))))
+    (A.varray (A.split_r slab_region (u32_to_sz (U32.mul (G.reveal x') page_size))) `star`
+    A.varray (A.split_r md_bm_region (u32_to_sz (U32.mul (G.reveal x') 4ul))) `star`
+    A.varray (A.split_r md_region (u32_to_sz (G.reveal x'))));
+
+  // change_slprop_rel
+  //   (A.varray (A.split_r slab_region (u32_to_sz (U32.mul (G.reveal x) page_size))) `star`
+  //   A.varray (A.split_r md_bm_region (u32_to_sz (U32.mul (G.reveal x) 4ul))) `star`
+  //   A.varray (A.split_r md_region (u32_to_sz (G.reveal x))))
+  //   (A.varray (A.split_r slab_region (u32_to_sz (U32.mul (G.reveal x') page_size))) `star`
+  //   A.varray (A.split_r md_bm_region (u32_to_sz (U32.mul (G.reveal x') 4ul))) `star`
+  //   A.varray (A.split_r md_region (u32_to_sz (G.reveal x'))))
+  //   (fun x y -> x == y)
+  //   (fun _ -> admit ());
+  let r = alloc_metadata size_class slab_region md_bm_region md_region md_count x' in
+  //TODO: hideous coercion that leads to 2 change_slprop_rel
+  change_equal_slprop
+    (A.varray (A.split_r slab_region (u32_to_sz (U32.mul (U32.add (G.reveal x') 1ul) page_size))) `star`
+    A.varray (A.split_r md_bm_region (u32_to_sz (U32.mul (U32.add (G.reveal x') 1ul) 4ul))) `star`
+    A.varray (A.split_r md_region (u32_to_sz (U32.add (G.reveal x') 1ul))))
+    (A.varray (A.split_r slab_region (u32_to_sz (U32.mul (U32.add (G.reveal x) 1ul) page_size))) `star`
+    A.varray (A.split_r md_bm_region (u32_to_sz (U32.mul (U32.add (G.reveal x) 1ul) 4ul))) `star`
+    A.varray (A.split_r md_region (u32_to_sz (U32.add (G.reveal x) 1ul))));
+  intro_vrefinedep
+    (vptr md_count)
+    (fun x -> U32.v x <= U32.v metadata_max == true)
+    (fun v ->
+      A.varray (A.split_r slab_region (u32_to_sz (U32.mul v page_size))) `star`
+      A.varray (A.split_r md_bm_region (u32_to_sz (U32.mul v 4ul))) `star`
+      A.varray (A.split_r md_region (u32_to_sz v)))
+    (A.varray (A.split_r slab_region (u32_to_sz (U32.mul (U32.add (G.reveal x) 1ul) page_size))) `star`
+      A.varray (A.split_r md_bm_region (u32_to_sz (U32.mul (U32.add (G.reveal x) 1ul) 4ul))) `star`
+      A.varray (A.split_r md_region (u32_to_sz (U32.add (G.reveal x) 1ul))));
+  return (fst r)
+#pop-options
+
+//assume val alloc_metadata3
+//  (size_class: sc)
+//  (slab_region: array U8.t{A.length slab_region = U32.v metadata_max * U32.v page_size})
+//  (md_bm_region: array U64.t{A.length md_bm_region = U32.v metadata_max * 4})
+//  (md_region: array (SL.cell blob){A.length md_region = U32.v metadata_max})
+//  (md_count: ref U32.t)
+//  : Steel (SL.t blob)
+//  //: Steel unit
+//  (
+//    vrefinedep
+//      (vptr md_count)
+//      (fun x -> U32.v x < U32.v metadata_max == true)
+//      (fun v ->
+//        A.varray (A.split_r slab_region (u32_to_sz (U32.mul v page_size))) `star`
+//        A.varray (A.split_r md_bm_region (u32_to_sz (U32.mul v 4ul))) `star`
+//        A.varray (A.split_r md_region (u32_to_sz v)))
+//  )
+//  (fun r ->
+//    SL.llist (p_empty size_class) r `star`
+//    vrefinedep
+//      (vptr md_count)
+//      (fun x -> U32.v x <= U32.v metadata_max == true)
+//      (fun v ->
+//        A.varray (A.split_r slab_region (u32_to_sz (U32.mul v page_size))) `star`
+//        A.varray (A.split_r md_bm_region (u32_to_sz (U32.mul v 4ul))) `star`
+//        A.varray (A.split_r md_region (u32_to_sz v)))
+//  )
+//  (requires fun h0 -> True)
+//  (ensures fun h0 r h1 ->
+//    //TODO FIXME: fails with this postcondition
+//    //L.length (SL.v_llist (p_empty size_class) r h1) = 1
+//    ///\ sel md_count h1 = U32.add (sel md_count h0) 1ul
+//  )
